theories/logrel/fundamental.v
@@ -1,0 +1,39 @@
+From iris.proofmode Require Import tactics.
+From machine_program_logic.program_logic Require Import weakestpre.
+From HypVeri.lang Require Import lang.
+From HypVeri.algebra Require Import base.
+From HypVeri.rules Require Import rules_base.
+From HypVeri.logrel Require Import logrel.
+Import uPred.
+
+Section fundamental.
+  Context `{hypconst:HypervisorConstants}.
+  Context `{hypparams:!HypervisorParameters}.
+  Context `{vmG: !gen_VMG Σ}.
+
+  (* Global Instance VMProp_timeless id Q q: Timeless (VMProp id Q q). *)
+  (* Proof. rewrite /VMProp. admit.  Admitted. *)
+
+  Lemma ftlr (i:VMID) (pgt:page_table) (regs: reg_file):
+    interp_access i pgt regs⊢ interp_execute i.
+  Proof.
+    rewrite /interp_access /=.
+    iIntros "((%Hreg_full & regs) & VMProp) Hnotp VMProp_holds".
+    iDestruct (VMProp_holds_agree i with "[VMProp_holds VMProp]") as "[Hres VMProp]".
+    { iFrame. }
+    iDestruct( later_or with "Hres") as "Hres".
+    iDestruct "Hres" as "[Hres| >False]";last done.
+    { (* the vm is scheduled *)
+      rewrite !later_sep.
+      (* we have to do this because VMProp is not(?) timeless *)
+      iDestruct "Hres" as "(>R0z & >R1z & VMPropz)".
+      (* getting the PC *)
+      pose proof (Hlookup_PC:= (Hreg_full PC)).
+      simpl in Hlookup_PC.
+      destruct Hlookup_PC as [ai Hlookup_PC].
+      rewrite (big_opM_delete _ _ PC ai Hlookup_PC).
+      iDestruct ("regs") as "[PC regs]".
+
+    }
+
+End fundamental.
